\chapter{The Superstition of Waves}

\section{The Addition of Waves}

\subsection{The Algebraic Method}

\begin{equation*}
  \begin{aligned}
    E \left( x, t \right) = E_0 \sin \left[ \omega t - \left( k x + \varepsilon \right) \right]
  \end{aligned}
\end{equation*}

let

\begin{equation*}
  \begin{aligned}
    \alpha \left( x , \varepsilon \right) = - \left( k x + \varepsilon \right)
  \end{aligned}
\end{equation*}

Then

\begin{equation*}
  \begin{aligned}
    E \left( x , t \right) = E_0 \sin \left[ \omega t + \alpha \left( x , \varepsilon \right) \right]
  \end{aligned}
\end{equation*}

Two waves of the same frequency

\begin{equation*}
  \left\{
    \begin{aligned}
      & E_1 = E_{01} \sin \left( \omega t + \alpha_1 \right) \\
      & E_2 = E_{02} \sin \left( \omega t + \alpha_2 \right) 
    \end{aligned}
  \right.
\end{equation*}

\begin{equation*}
  \begin{aligned}
    E = E_1 + E_2 &= E_{01} \left( \sin \omega t \cos \alpha_1 + \cos \omega t \sin \alpha_1 \right) + E_{02} \left( \sin \omega t \cos \alpha_2 + \cos \omega t \sin \alpha_2  \right) \\
    &= \left( E_{01} \cos \alpha_1 + E_{02} \cos \alpha_2 \right) \sin \omega t + \left( E_{01} \sin \alpha_1 + E_{02} \sin \alpha_2 \right) \cos \omega t \\
    &= E_0 \cos \alpha \sin \omega t + E_0 \sin \alpha \cos \omega t \\
    &= E_0 \sin \left( \omega t + \alpha \right)
  \end{aligned}
\end{equation*}

\begin{equation*}
  \left\{
    \begin{aligned}
      & E_0 \cos \alpha = E_{01} \cos \alpha_1 + E_{02} \cos \alpha_2 \\
      & E_0 \sin \alpha = E_{01} \sin \alpha_1 + E_{02} \sin \alpha_2 \\
    \end{aligned}
  \right.
  \Rightarrow
  \left\{
    \begin{aligned}
      & E_0^2 = E_{01}^2 + E_{02}^2 + 2 E_{01} E_{02} \cos \left( \alpha_2 - \alpha_1 \right) \\
      & \tan \alpha = \dfrac{E_{01} \sin \alpha_1 + E_{02} \sin \alpha_2}{E_{01} \cos \alpha_1 + E_{02} \cos \alpha_2} 
    \end{aligned}
  \right.
\end{equation*}

The phase difference

\begin{equation*}
  \begin{aligned}
    \delta = \left( k x_1 + \varepsilon_1 \right) - \left( k x_2 + \varepsilon_2 \right) = \dfrac{2 \pi}{\lambda} \left( x_1 - x_2 \right) + \left( \varepsilon_1 - \varepsilon_2 \right)
  \end{aligned}
\end{equation*}

When $E_{01} = E_{02}$ and $\alpha_2 - \alpha_1 = \Delta x$
\begin{equation*}
  \begin{aligned}
      & E_0^2 = 2 E_{01}^2 + 2 E_{01}^2 \cos \left( k \Delta x \right) = 2 E_{01}^2 \left[ 1 + \cos \left( k \Delta x \right) \right] \\
  \end{aligned}
\end{equation*}

\begin{equation*}
  \begin{aligned}
    \cos 2x = 2 \cos^2 x - 1 \Rightarrow \cos \left( k \Delta x \right) = 2 \cos^2 \left( \dfrac{k \Delta x}{2}  \right) - 1
  \end{aligned}
\end{equation*}

$\Rightarrow$

\begin{equation*}
  \begin{aligned}
    E_0^2 = 2 E_{01}^2 \cos^2 \left( \dfrac{k \Delta x}{2}  \right)
  \end{aligned}
\end{equation*}

Period of the amplitude of addition

\begin{equation*}
  \begin{aligned}
    \dfrac{k \Delta x}{2} = \dfrac{\pi}{2}  \Rightarrow k \left( \alpha_2 - \alpha_1 \right) = \pi \Rightarrow \Delta x = \alpha_2 - \alpha_1 = \dfrac{\lambda}{2} 
  \end{aligned}
\end{equation*}



%%% Local Variables:
%%% mode: latex
%%% TeX-master: "Optics"
%%% End:
